Tap

DLCF/Typing/Subst.lean
@@ -8,14 +8,16 @@ variable {Λ} [DecidableEq Λ] [Level Λ] [maxU : LevelBound Λ]
 
 structure FSubst.JEq (Γ Δ : Finset (FVar Λ)) (σ σ' : FSubst Λ) : Prop where
   okIn : Ok Γ
-  jeq : ∀x ∈ Δ, Γ ⊢ σ x ≡ σ' x : x.ty
+  jeq : ∀x ∈ Δ, Γ ⊢ σ x ≡ σ' x : x.ty.fsubst σ
 
 notation Γ " ⊢ " a " ≡ " b " ▷ " Δ => FSubst.JEq Γ Δ a b
 
-theorem FSubst.JEq.symm {Γ Δ : Finset (FVar Λ)} {σ σ' : FSubst Λ} (h : Γ ⊢ σ ≡ σ' ▷ Δ)
-  : Γ ⊢ σ' ≡ σ ▷ Δ where
-  okIn := h.okIn
-  jeq x hx := (h.jeq x hx).symm
+-- TODO: proving this requires regularity ... or do we do the HEq trick?
+-- _or_ can prove jeq_right by induction?
+-- theorem FSubst.JEq.symm {Γ Δ : Finset (FVar Λ)} {σ σ' : FSubst Λ} (h : Γ ⊢ σ ≡ σ' ▷ Δ)
+--   : Γ ⊢ σ' ≡ σ ▷ Δ where
+--   okIn := h.okIn
+--   jeq x hx := (h.jeq x hx).symm
 
 theorem FSubst.JEq.trans {Γ Δ : Finset (FVar Λ)} {σ σ' σ'' : FSubst Λ}
   (h : Γ ⊢ σ ≡ σ' ▷ Δ) (h' : Γ ⊢ σ' ≡ σ'' ▷ Δ) : Γ ⊢ σ ≡ σ'' ▷ Δ where
@@ -41,34 +43,54 @@ theorem FSubst.JEq.empty {Γ : Finset (FVar Λ)} {σ σ' : FSubst Λ} (hΓ : Ok 
 theorem FSubst.JEq.empty_iff {Γ : Finset (FVar Λ)} {σ σ' : FSubst Λ}
   : (Γ ⊢ σ ≡ σ' ▷ ∅) ↔ Ok Γ := ⟨λh => h.okIn, λh => empty h⟩
 
-theorem FSubst.JEq.insert {Γ Δ : Finset (FVar Λ)} {σ σ' : FSubst Λ} {x : FVar Λ}
-  (h : Γ ⊢ σ ≡ σ' ▷ Δ) (hx : Γ ⊢ σ x ≡ σ' x : x.ty) : Γ ⊢ σ ≡ σ' ▷ insert x Δ where
+theorem FSubst.JEq.insertIn {Γ Δ : Finset (FVar Λ)} {σ σ' : FSubst Λ}
+  (hA : Γ ⊢ A ≡ A : .univ n) (h : Γ ⊢ σ ≡ σ' ▷ Δ) : (insert ⟨i, A⟩ Γ) ⊢ σ ≡ σ' ▷ Δ where
+  okIn := hA.ok_var i
+  jeq y hy := (h.jeq y hy).wki hA
+
+theorem FSubst.JEq.insertOut {Γ Δ : Finset (FVar Λ)} {σ σ' : FSubst Λ} {x : FVar Λ}
+  (h : Γ ⊢ σ ≡ σ' ▷ Δ) (hx : Γ ⊢ σ x ≡ σ' x : x.ty.fsubst σ) : Γ ⊢ σ ≡ σ' ▷ insert x Δ where
   okIn := h.okIn
   jeq y hy := if hxy : y = x then hxy ▸ hx else h.jeq y (Finset.mem_of_mem_insert_of_ne hy hxy)
 
-theorem FSubst.JEq.insert_jeq {Γ Δ : Finset (FVar Λ)} {σ σ' : FSubst Λ} {x : FVar Λ}
-  (h : Γ ⊢ σ ≡ σ' ▷ (Insert.insert x Δ)) : Γ ⊢ σ x ≡ σ' x : x.ty
+theorem FSubst.JEq.insertOut_jeq {Γ Δ : Finset (FVar Λ)} {σ σ' : FSubst Λ} {x : FVar Λ}
+  (h : Γ ⊢ σ ≡ σ' ▷ (Insert.insert x Δ)) : Γ ⊢ σ x ≡ σ' x : x.ty.fsubst σ
   := h.jeq x (Finset.mem_insert_self x Δ)
 
-theorem FSubst.JEq.insert_rest {Γ Δ : Finset (FVar Λ)} {σ σ' : FSubst Λ} {x : FVar Λ}
+theorem FSubst.JEq.insertOut_rest {Γ Δ : Finset (FVar Λ)} {σ σ' : FSubst Λ} {x : FVar Λ}
   (h : Γ ⊢ σ ≡ σ' ▷ (Insert.insert x Δ)) : Γ ⊢ σ ≡ σ' ▷ Δ := h.wkOut (Finset.subset_insert x Δ)
 
-theorem FSubst.JEq.insert_iff {Γ Δ : Finset (FVar Λ)} {σ σ' : FSubst Λ} {x : FVar Λ}
-  : (Γ ⊢ σ ≡ σ' ▷ (Insert.insert x Δ)) ↔ (Γ ⊢ σ x ≡ σ' x : x.ty) ∧ (Γ ⊢ σ ≡ σ' ▷ Δ)
-  := ⟨λh => ⟨h.insert_jeq, h.insert_rest⟩, λ⟨h, h'⟩ => h'.insert h⟩
+theorem FSubst.JEq.insertOut_iff {Γ Δ : Finset (FVar Λ)} {σ σ' : FSubst Λ} {x : FVar Λ}
+  : (Γ ⊢ σ ≡ σ' ▷ (Insert.insert x Δ)) ↔ (Γ ⊢ σ x ≡ σ' x : x.ty.fsubst σ) ∧ (Γ ⊢ σ ≡ σ' ▷ Δ)
+  := ⟨λh => ⟨h.insertOut_jeq, h.insertOut_rest⟩, λ⟨h, h'⟩ => h'.insertOut h⟩
+
+-- theorem JEq.subst {Γ Δ : Finset (FVar Λ)} (hσ : Γ ⊢ σ ≡ σ' ▷ Δ) (ha : Δ ⊢ a ≡ a' : A)
+--   : Γ ⊢ a.fsubst σ ≡ a'.fsubst σ' : A.fsubst σ := by induction ha with
+--   | top_emp => exact hσ.okIn.top
+--   | top_cons => exact hσ.okIn.top
+--   | var hA hx IA => exact hσ.jeq _ hx
+--   | bot => exact hσ.okIn.bot
+--   | tt => exact hσ.okIn.tt
+--   | dite hφ ht hf Iφ It If =>
+--     apply JEq.dite (Iφ hσ)
+--     sorry
+--     sorry
+--   | _ =>
+--     constructor
+--     <;> sorry
 
 -- TODO: add induction principle for FSubst...
 
 -- TODO: insert set, based on ⊥ and friends...
 
 theorem FSubst.JEq.singleton {Γ : Finset (FVar Λ)} {σ σ' : FSubst Λ} {x : FVar Λ}
-  (h : Γ ⊢ σ x ≡ σ' x : x.ty) : Γ ⊢ σ ≡ σ' ▷ {x} := (empty h.ok).insert h
+  (h : Γ ⊢ σ x ≡ σ' x : x.ty.fsubst σ) : Γ ⊢ σ ≡ σ' ▷ {x} := (empty h.ok).insertOut h
 
 theorem FSubst.JEq.singleton_jeq {Γ : Finset (FVar Λ)} {σ σ' : FSubst Λ} {x : FVar Λ}
-  (h : Γ ⊢ σ ≡ σ' ▷ {x}) : Γ ⊢ σ x ≡ σ' x : x.ty := h.jeq x (Finset.mem_singleton_self x)
+  (h : Γ ⊢ σ ≡ σ' ▷ {x}) : Γ ⊢ σ x ≡ σ' x : x.ty.fsubst σ := h.jeq x (Finset.mem_singleton_self x)
 
 theorem FSubst.JEq.singleton_iff {Γ : Finset (FVar Λ)} {σ σ' : FSubst Λ} {x : FVar Λ}
-  : (Γ ⊢ σ ≡ σ' ▷ {x}) ↔ (Γ ⊢ σ x ≡ σ' x : x.ty) := ⟨singleton_jeq, singleton⟩
+  : (Γ ⊢ σ ≡ σ' ▷ {x}) ↔ (Γ ⊢ σ x ≡ σ' x : x.ty.fsubst σ) := ⟨singleton_jeq, singleton⟩
 
 theorem FSubst.JEq.union {Γ Δ Δ' : Finset (FVar Λ)} {σ σ' : FSubst Λ}
   (h : Γ ⊢ σ ≡ σ' ▷ Δ) (h' : Γ ⊢ σ ≡ σ' ▷ Δ') : Γ ⊢ σ ≡ σ' ▷ Δ ∪ Δ' where
@@ -78,10 +100,11 @@ theorem FSubst.JEq.union {Γ Δ Δ' : Finset (FVar Λ)} {σ σ' : FSubst Λ}
     · apply h.jeq; assumption
     · apply h'.jeq; assumption
 
-theorem FSubst.JEq.left_congr_trg {Γ Δ : Finset (FVar Λ)} {σ σ' τ : FSubst Λ}
-  (hσ : ∀x ∈ Δ, σ x = τ x) (h : Γ ⊢ σ ≡ σ' ▷ Δ) : Γ ⊢ τ ≡ σ' ▷ Δ where
-  okIn := h.okIn
-  jeq x hx := hσ x hx ▸ h.jeq x hx
+-- TODO: need regularity for this too, unless, again, HEq trick
+-- theorem FSubst.JEq.left_congr_trg {Γ Δ : Finset (FVar Λ)} {σ σ' τ : FSubst Λ}
+--   (hσ : ∀x ∈ Δ, σ x = τ x) (h : Γ ⊢ σ ≡ σ' ▷ Δ) : Γ ⊢ τ ≡ σ' ▷ Δ where
+--   okIn := h.okIn
+--   jeq x hx := hσ x hx ▸ h.jeq x hx
 
 theorem FSubst.JEq.right_congr_trg {Γ Δ : Finset (FVar Λ)} {σ σ' τ : FSubst Λ}
   (hσ' : ∀x ∈ Δ, σ' x = τ x) (h : Γ ⊢ σ ≡ σ' ▷ Δ) : Γ ⊢ σ ≡ τ ▷ Δ where
@@ -91,7 +114,7 @@ theorem FSubst.JEq.right_congr_trg {Γ Δ : Finset (FVar Λ)} {σ σ' τ : FSubs
 structure FSubst.Wf (Γ Δ : Finset (FVar Λ)) (σ : FSubst Λ) : Prop where
   okIn : Ok Γ
   okOut : Ok Δ
-  wf : ∀x ∈ Δ, Γ ⊢ σ x : x.ty
+  wf : ∀x ∈ Δ, Γ ⊢ σ x : x.ty.fsubst σ
 
 notation Γ " ⊢ " a " ▷ " Δ => FSubst.Wf Γ Δ a
 
