DLCF/Typing/Basic.lean
@@ -68,6 +68,15 @@ theorem JEq.to_top (h : Γ ⊢ a ≡ b : A) : Γ ⊢ ⊤ ≡ ⊤ : .univ 0
   | top_cons hA => exact .top_cons hA
   | _ => assumption
 
+-- theorem JEq.sides_lc (h : Γ ⊢ a ≡ b : A) : a.bv = 0 ∧ b.bv = 0 := by
+--   induction h with
+--   | dite => sorry
+--   | pi => sorry
+--   | abs => sorry
+--   | app => sorry
+--   | β_abs => sorry
+--   | _ => simp [bv, *]
+
 -- theorem JEq.sides_valid (h : Γ ⊢ a ≡ b : A) : a.valid ∧ b.valid := by
 --   induction h <;> simp [valid, bsubst0_valid_iff, *] at *
 --   sorry
